#Übung 
#GMI 
#Medieninformatik 

---
![[Pasted image 20221124133652.png]]

# Aufgabe 20
## 20.1
a) $2x$
$f'(x)=\lim_{ h \to 0 } \frac{f(x_{0}+h)-f(x_{0})}{h}=\frac{(x_{0}+h)^{2}+5-x_{0}^2-5}{h}=\frac{(x_{0}+h)^{2}-x_{0}^2}{h}=\frac{x_{0}^2+2x_{0}h+h^2-x_{0}^2}{h}=\frac{2x_{0}h+h^2}{h}=\frac{x_{0}^2+2x_{0}h+h^2-x_{0}^2}{h}$
$=\frac{h(2x_{0}+h)}{h}= 2x_{0}+0=2x$


b)
$3x^{2}+3$

$f'(x)=\lim_{ h \to 0 } \frac{((x_{0}+h)^3+3(x_{0}+h))-(x_{0}^3+3x_{0})}{h}=\frac{(((x_{0}+h)^2*(x_{0}+h))+3(x_{0}+h))-(x_{0}^3+3x_{0})}{h}=\frac{(x_{0}^2+2x_{0}h+h^{2})(x_{0}+h)+3(x_{0}+h)-(x_{0}^3+3x_{0})}{h}$
$= \frac{(x_{0}^2+2x_{0}h+h^{2})(x_{0}+h)+3x_{0}+3h-x_{0}^3-3x_{0}}{h}$

$=\frac{x_{0}^3+x_{0}^{2}h+2x_{0}^{2}h+2x_{0}h^{2}+h^{2}x_{0}+h^{3}+3h-x_{0}^3}{h}$

$= \frac{x_{0}^{2}h+2x_{0}^{2}h+3x_{0}h^{2}+h^{3}+3h}{h}$

![[Pasted image 20221124144525.png]]

# Aufgabe 22
![[Pasted image 20221124144722.png]]
![[Pasted image 20221124144455.png]]

# Aufgabe 23

# Mitschrieb
![[Notiz 24.11.2022 Ü.pdf]]
